tla/MC_ConcurrentBumpFreshOnly.tla
@@ -1,0 +1,3 @@
+---------------------- MODULE MC_ConcurrentBumpFreshOnly ----------------------
+EXTENDS ConcurrentBumpFreshOnly
+=============================================================================
